intermediate/Veritas.Intermediate.Store.fsti
@@ -10,7 +10,6 @@ module FE = FStar.FunctionalExtensionality
 
 (*** General Definitions & Basic Facts ***)
 
-let slot_id = nat
 let add_method = Veritas.Verifier.add_method
 
 (* 
@@ -21,84 +20,181 @@ type vstore_entry =
   | VStoreE: k:key -> 
              v:value_type_of k -> 
              am:add_method -> 
-             l_in_store : option slot_id{is_merkle_key k \/ None = l_in_store} -> 
-             r_in_store : option slot_id{is_merkle_key k \/ None = r_in_store} -> 
+             l_in_store : option nat{is_merkle_key k \/ None = l_in_store} -> 
+             r_in_store : option nat{is_merkle_key k \/ None = r_in_store} -> 
              vstore_entry
 
-(* vstore: None => entry is currently not occupied *)
-type vstore = Seq.seq (option vstore_entry) 
+(* vstore_raw: the raw version of the vstore; the actual vstore 
+ * is the raw version with some invariants *)
+type vstore_raw = Seq.seq (option vstore_entry) 
 
-let empty_store (n:nat) :vstore = Seq.create n None
+(* an index in store *)
+let slot_id (st:vstore_raw) = seq_index st
 
-let st_index (st:vstore) = seq_index st
-
-let get_slot (st:vstore) (s:slot_id)
+let get_slot (st:vstore_raw) (s: slot_id st)
   : option vstore_entry
-  = if s >= Seq.length st then None else Seq.index st s
+  = Seq.index st s
 
 (* return true if s is a valid slot that is occupied *)
-let store_contains (st:vstore) (s:slot_id) : bool
+let inuse_slot (st:vstore_raw) (s:slot_id st) : bool
   = Some? (get_slot st s)
 
-let store_contains_st_index (st:vstore) (s:slot_id{store_contains st s})
-  : Lemma (s < Seq.length st)
-          [SMTPat (store_contains st s)] 
-  = ()
+(* dep type of all slots in use *)
+let inuse_slot_id (st: vstore_raw) = s:slot_id st{inuse_slot st s}
 
-let lemma_store_contains_empty (n:nat) (s:slot_id)
-  : Lemma (not (store_contains (empty_store n) s))
-          [SMTPat (store_contains (empty_store n) s)]
-  = ()
+let get_inuse_slot (st:vstore_raw) (s:inuse_slot_id st) =
+  Some?.v (get_slot st s)
+
+(* is this an empty slot *)
+let empty_slot (st:vstore_raw) (s:slot_id st): bool 
+  = None = get_slot st s
+
+let empty_slot_id (st: vstore_raw) = s:slot_id st{empty_slot st s}
 
 (* key stored at an occupied slot *)
-let stored_key (st:vstore) (s:slot_id{store_contains st s}) : key
+let stored_key (st:vstore_raw) (s:inuse_slot_id st) : key
   = VStoreE?.k (Some?.v (get_slot st s))
 
-let stored_value (st:vstore) (s:slot_id{store_contains st s}) : value
+(* is this a slot containing a merkle key *)
+let merkle_slot_id (st:vstore_raw)
+  = s:inuse_slot_id st{is_merkle_key (stored_key st s)}
+
+let data_slot_id (st:vstore_raw)
+  = s:inuse_slot_id st{is_data_key (stored_key st s)}
+
+let stored_value (st:vstore_raw) (s:inuse_slot_id st) : value
   = VStoreE?.v (Some?.v (get_slot st s))
 
-let stored_value_matches_stored_key (st:vstore) (s:slot_id{store_contains st s}) 
-  : Lemma (is_value_of (stored_key st s) (stored_value st s))
-    [SMTPat (is_value_of (stored_key st s) (stored_value st s))]
-  = ()
-
-let add_method_of (st:vstore) (s:slot_id{store_contains st s}) : add_method
+let add_method_of (st:vstore_raw) (s:inuse_slot_id st) : add_method
   = VStoreE?.am (Some?.v (get_slot st s))
-  
-(* is this a slot containing a merkle key *)
-type instore_merkle_slot (st:vstore)
-  = s:slot_id {store_contains st s /\ is_merkle_key (stored_key st s)}
+
+(* TODO: Move to a better place ?*)
+let mv_points_to_none (mv:merkle_value) (d:bin_tree_dir): bool 
+  = Empty? (desc_hash_dir mv d)
+
+let mv_points_to_some (mv:merkle_value) (d:bin_tree_dir) : bool
+  = Desc? (desc_hash_dir mv d)
+
+let mv_pointed_key (mv:merkle_value) (d:bin_tree_dir{mv_points_to_some mv d}) : key
+  = Desc?.k (desc_hash_dir mv d)
 
 (* was a descendant added with MAdd along direction d *)
-let desc_in_store (st:vstore) (s:instore_merkle_slot st) (d:bin_tree_dir) : bool
+let desc_in_store (st:vstore_raw) (s:inuse_slot_id st) (d:bin_tree_dir) : bool
   = match d with
     | Left -> Some? (VStoreE?.l_in_store (Some?.v (get_slot st s)))
     | Right -> Some? (VStoreE?.r_in_store (Some?.v (get_slot st s)))
 
 (* if a descendant was added with MAdd, the slot where the descendant was added *)
-let desc_slot (st:vstore) (s:instore_merkle_slot st) (d:bin_tree_dir{desc_in_store st s d}): slot_id
+let desc_slot (st:vstore_raw) (s:inuse_slot_id st) (d:bin_tree_dir{desc_in_store st s d}): nat
   = match d with
     | Left -> Some?.v (VStoreE?.l_in_store (Some?.v (get_slot st s)))
     | Right -> Some?.v (VStoreE?.r_in_store (Some?.v (get_slot st s)))
 
+(* invariant connecting the value stored in a slot and the desc info *)
+let desc_in_store_inv_merkle (st:vstore_raw) (s:merkle_slot_id st) (d:bin_tree_dir) = 
+  let v = to_merkle_value (stored_value st s) in
+  mv_points_to_none v d /\ not (desc_in_store st s d) \/
+  mv_points_to_some v d /\ (desc_in_store st s d ==> 
+                            (let ds = desc_slot st s d in
+                             ds < Seq.length st /\               // valid slot_id                 
+                             (let dk = mv_pointed_key v d in
+                              inuse_slot st ds /\                // slot_id in use                              
+                              stored_key st ds = dk /\           // stored key is the key in my value
+                              add_method_of st ds = Spec.MAdd))) // Merkle add
+
+let desc_in_store_inv_data (st:vstore_raw) (s:data_slot_id st) = 
+  not (desc_in_store st s Left) && 
+  not (desc_in_store st s Right)
+
+let store_inv_slot (st:vstore_raw) (s:slot_id st) = 
+  empty_slot st s \/
+  (is_data_key (stored_key st s) /\ desc_in_store_inv_data st s) \/
+  (is_merkle_key (stored_key st s) /\ 
+   desc_in_store_inv_merkle st s Left /\ 
+   desc_in_store_inv_merkle st s Right)
+
+let store_inv_local (st:vstore_raw) = 
+  forall (s:slot_id st). store_inv_slot st s
+
+let vstore = st:vstore_raw{store_inv_local st}
+
+let empty_store (n:nat) :vstore = Seq.create n None
+  
 let has_key (k:key) (e:option vstore_entry) : bool
   = match e with
     | Some (VStoreE k' _ _ _ _) -> k = k'
     | None -> false
 
-let update_slot (st:vstore) (s:st_index st) (e:vstore_entry)
-  : vstore
-  = Seq.upd st s (Some e)
+(** vstore update methods **)
+
+(* relationship between two stores st and st' that states that 
+ * they are of the same size and differ in only one slot *)
+let idx_store_update_rel (st st': vstore) (s:slot_id st) 
+  = Seq.length st = Seq.length st' /\
+    (forall (s':slot_id st). (s' <> s ==> get_slot st s' == get_slot st' s'))
+
+(* add a new entry (k,v) to the store at en empty slot s; *)
+val add_to_store 
+      (st:vstore) 
+      (s:empty_slot_id st)
+      (k:key) 
+      (v:value_type_of k) 
+      (am:add_method)
+  : Tot (st':vstore {idx_store_update_rel st st' s /\
+                     inuse_slot st' s /\
+                     get_inuse_slot st' s = VStoreE k v am None None})
+
+(* add a new entry with merkle and a descendant *)
+(* TODO: Add when this is used *)
+val add_to_store_with_desc
+      (st:vstore)
+      (s:empty_slot_id st)
+      (k:merkle_key)
+      (v:merkle_value)
+      (d:bin_tree_dir{mv_points_to_some v d})
+      (s':merkle_slot_id st{mv_pointed_key v d = stored_key st s'})
+  : Tot (st':vstore {idx_store_update_rel st st' s /\
+                     inuse_slot st' s /\
+                     stored_key st' s = k /\
+                     stored_value st' s = (MVal v) /\
+                     add_method_of st' s = Spec.MAdd /\
+                     desc_in_store st' s d /\
+                     desc_slot st' s d = s' /\
+                     not (desc_in_store st' s d)})
+                     
+(* update the data value of a data key *)
+val update_data_value 
+  (st:vstore)
+  (s:data_slot_id st)
+  (v:value{DVal? v})
+  : Tot (st':vstore {idx_store_update_rel st st' s /\
+                     inuse_slot st' s /\
+                     stored_key st' s = stored_key st s /\                     
+                     stored_value st' s = v})
+
+(* reset a descendant of a merkle slot *)
+val reset_desc_slot
+  (st:vstore)
+  (s:merkle_slot_id st)
+  (d:bin_tree_dir{desc_in_store st s d})
+  : Tot (st': vstore {Seq.length st = Seq.length st' /\
+                      inuse_slot st' s /\ 
+                      stored_key st' s = stored_key st s /\
+                      not (desc_in_store st s d)})
+
 
 (* update the value of an occupied store slot with a compatible value *)
 let update_value 
   (st:vstore)
-  (s:slot_id{store_contains st s}) 
+  (s:inuse_slot_id st) 
   (v:value_type_of (stored_key st s))
-  : Tot (st':vstore {store_contains st' s /\
+  : Tot (st':vstore {Seq.length st = Seq.length st' /\
+                     inuse_slot st' s /\
                      stored_value st' s = v})
   = let Some (VStoreE k _ am l r) = get_slot st s in
-    update_slot st s (VStoreE k v am l r)
+    let st' = update_slot st s (VStoreE k v am l r) in
+    admit()
+    //update_slot st s (VStoreE k v am l r)
 
 let update_value_preserves_length 
       (st:vstore) 
@@ -118,7 +214,7 @@ let lemma_update_value_preserves_slots
           [SMTPat (store_contains (update_value st s v) s')]
   = ()
 
-(* update desc in store *)
+(* update desc in store; we do not have an update that sets desc_in_store to None *)
 let update_desc_in_store
   (st:vstore)
   (s:instore_merkle_slot st)
@@ -133,33 +229,6 @@ let update_desc_in_store
     | Left -> update_slot st s (VStoreE k v am (Some s') rd) 
     | Right -> update_slot st s (VStoreE k v am ld (Some s'))
 
-(* update desc in store *)
-let reset_desc_in_store
-  (st:vstore)
-  (s:instore_merkle_slot st)
-  (d:bin_tree_dir)
-  : Tot (st':vstore {store_contains st' s /\ 
-                     stored_key st' s = stored_key st s /\
-                     not (desc_in_store st' s d)})
-  = let Some (VStoreE k v am ld rd) = get_slot st s in
-    match d with
-    | Left -> update_slot st s (VStoreE k v am None rd) 
-    | Right -> update_slot st s (VStoreE k v am ld None)
-
-(* add a new entry (k,v,am) to the store at en empty slot s 
-   --> this is the only function that may violate the is_map invariant (defined below) *)
-let add_to_store 
-      (st:vstore) 
-      (s:st_index st{not (store_contains st s)}) 
-      (k:key) 
-      (v:value_type_of k) 
-      (am:add_method)
-  : Tot (st':vstore {store_contains st' s /\
-                     stored_key st' s = k /\
-                     stored_value st' s = v /\
-                     add_method_of st' s = am})
-  = let e = VStoreE k v am None None in // default for desc_in_store is None (no desc)
-    update_slot st s e
 
 (* remove an entry from a slot; reset slot to unused *)
 let evict_from_store (st:vstore) (s:st_index st)
@@ -208,37 +277,13 @@ let elim_is_map (st:vstore)
           (ensures stored_key st s ≠ stored_key st s')
   = ()
 
-let mv_points_to_none (mv:merkle_value) (d:bin_tree_dir): bool 
-  = Empty? (desc_hash_dir mv d)
-
-let mv_points_to_some (mv:merkle_value) (d:bin_tree_dir) : bool
-  = Desc? (desc_hash_dir mv d)
-
 let points_to_some (st:vstore) (s:instore_merkle_slot st) (d:bin_tree_dir) : bool
   = let mv = to_merkle_value (stored_value st s) in
     mv_points_to_some mv d
 
-let mv_pointed_key (mv:merkle_value) (d:bin_tree_dir{mv_points_to_some mv d}) : key
-  = Desc?.k (desc_hash_dir mv d)
-
 let pointed_key (st:vstore) (s:instore_merkle_slot st) (d:bin_tree_dir{points_to_some st s d}) : key
   = let mv = to_merkle_value (stored_value st s) in
     mv_pointed_key mv d
-
-(* invariant connecting the value stored in a slot and the desc info *)
-let in_store_inv_slot (st:vstore) (s:instore_merkle_slot st) (d:bin_tree_dir) = 
-  let v = to_merkle_value (stored_value st s) in
-  mv_points_to_none v d /\ not (desc_in_store st s d) \/
-  mv_points_to_some v d /\ (desc_in_store st s d ==> 
-                            (let ds = desc_slot st s d in
-                             let dk = mv_pointed_key v d in
-                             store_contains st ds /\
-                             stored_key st ds = dk))
-
-let in_store_inv (st:vstore) 
-  = forall (s:instore_merkle_slot st) (d:bin_tree_dir).
-          {:pattern (in_store_inv_slot st s d)}
-    in_store_inv_slot st s d
 
 let store_inv (st:vstore) = 
   is_map st /\ in_store_inv st
@@ -254,12 +299,12 @@ let lemma_update_value_preserves_is_map
 
 let lemma_update_in_store_preserves_is_map
       (st:vstore) 
-      (s:slot_id{store_contains st s}) 
+      (s:instore_merkle_slot st) 
       (d:bin_tree_dir)
-      (b:bool)
+      (s':slot_id)
   : Lemma (requires (is_map st))
-          (ensures (is_map (update_in_store st s d b)))
-          [SMTPat (is_map (update_in_store st s d b))]
+          (ensures (is_map (update_desc_in_store st s d s')))
+          [SMTPat (is_map (update_desc_in_store st s d s'))]
   = ()
 
 (* is_map is preserved when adding a new key *)
@@ -422,7 +467,7 @@ val lemma_store_rel_contains_key (st:vstore) (st':Spec.vstore) (k:key)
           (ensures (store_contains_key st k = Spec.store_contains st' k))
           [SMTPat (store_contains_key st k); SMTPat (Spec.store_contains st' k)]
 
-val lemma_store_rel_stored_value (st:vstore) (st':Spec.vstore) (k:key)
+val lemma_store_rel_stored_value (st:vstore) (st':Spec.vstore) (k:key)
   : Lemma (requires (store_rel st st' /\ store_contains_key st k))
           (ensures (stored_value_by_key st k = Spec.stored_value st' k))
           [SMTPat (stored_value_by_key st k); SMTPat (Spec.stored_value st' k)]
